VsaIris.lean
@@ -69,6 +69,7 @@ import VsaIris.Interp.EnvGetSpans
 import VsaIris.Interp.EnvGetHit
 import VsaIris.Interp.EnvSetSpans
 import VsaIris.Interp.EnvSetHit
+import VsaIris.Interp.EnvDefineSpans
 import VsaIris.Interp.EnvScan
 import VsaIris.Interp.ProofEnvGet
 import VsaIris.Interp.ProofEnvSet
